remove quick cases and start Class -> DataType changes

SlowTest/ExtensibleArray-seq.dfy
@@ -1,125 +1,208 @@
 // RUN: %dafny /compile:0 /dprint:"%t.dprint" "%s" > "%t"
 // RUN: %diff "%s.expect" "%t"
 
-// datatype seq'<T> = Emp | NE(seq<T>)
-// function method seq_length<T> (s:seq'<T>):(n:int)
-//   requires s != Emp
-//   ensures match s case Emp => n == 0 case NE(s') => n == |s'|
+datatype Option<T> = Some(o: T) | None
+datatype Eseq<T> = Eseq(Contents: seq<T>, elements: Option< seq<T> >, more: Option< Eseq <seq<T> > >, length: int, M: int)
 
-// function method wrapper<T> (s:seq<T>):(s':seq'<T>)
-//   ensures if s == [] then s' == Emp else s' == NE(s)
+predicate Valid(s: Eseq)
+{
+  ( (s.elements == None && s.more == None && s.Contents == []) ||
+    (s.elements != None && |s.elements.o| == 256)
+  ) &&
 
-class ExtensibleArray<T> {
-  ghost var Contents: seq<T>
-  ghost var Repr: set<object?>
-  var elements: seq<T>
-  var more: ExtensibleArray?<seq<T>>
-  var length: int
-  var M: int  // shorthand for:  if more == null then 0 else 256 * |more.Contents|
+  ( s.more != None ==>
+    Valid (s.more.o) &&
+    |s.more.o.Contents| != 0 &&
+    forall j :: 0 <= j < |s.more.o.Contents| ==>
+      s.more.o.Contents[j] != [] && |s.more.o.Contents[j]| == 256 &&
+      s.more.o.Contents[j] != s.elements.o &&
+      forall k :: 0 <= k < |s.more.o.Contents| && k != j ==>
+        s.more.o.Contents[j] != s.more.o.Contents[k]
+  ) &&
 
-  predicate Valid()
-    reads this, Repr
+  // length
+  s.M == (if s.more == None then 0 else 256 * |s.more.o.Contents|) &&
+  0 <= s.length <= s.M + 256 &&
+  (s.more != None ==> s.M < s.length) &&
+
+  // Contents
+  s.length == |s.Contents| &&
+  (forall i :: 0 <= i < s.M ==> s.Contents[i] == s.more.o.Contents[i / 256][i % 256]) &&
+  (forall i :: s.M <= i < s.length ==> s.Contents[i] == s.elements.o[i - s.M])  
+}
+
+function Init<T>(): (s:Eseq<T>)
+  ensures Valid(s)
+  ensures s.Contents == []
+{
+  Eseq([], None, None, 0, 0)
+}
+
+method Get<T>(s: Eseq<T>, i: int) returns (t: T)
+  requires Valid(s)
+  requires 0 <= i < |s.Contents|
+  ensures t == s.Contents[i]
   {
-    // shape of data structure
-    this in Repr && null !in Repr &&
-    ((elements == [] && more == null && Contents == []) ||
-     (elements != [] && |elements| == 256 /*&& elements in Repr*/)) &&
-    (more != null ==>
-        more in Repr && more.Repr <= Repr && this !in more.Repr && /*elements !in more.Repr && */
-        more.Valid() &&
-        |more.Contents| != 0 &&
-        forall j :: 0 <= j < |more.Contents| ==>
-            more.Contents[j] != [] && |more.Contents[j]| == 256 &&
-            /* more.Contents[j] in Repr && more.Contents[j] !in more.Repr && */
-            more.Contents[j] != elements &&
-            forall k :: 0 <= k < |more.Contents| && k != j ==> more.Contents[j] != more.Contents[k]) &&
-
-    // length
-    M == (if more == null then 0 else 256 * |more.Contents|) &&
-    0 <= length <= M + 256 &&
-    (more != null ==> M < length) &&
-
-    // Contents
-    length == |Contents| &&
-    (forall i :: 0 <= i < M ==> Contents[i] == more.Contents[i / 256][i % 256]) &&
-    (forall i :: M <= i < length ==> Contents[i] == elements[i - M])
-  }
-
-  constructor Init()
-    ensures Valid() && fresh(Repr - {this})
-    ensures Contents == []
-  {
-    elements := [];
-    more := null;
-    length := 0;
-    M := 0;
-
-    Contents := [];
-    Repr := {this};
-  }
-
-  method Get(i: int) returns (t: T)
-    requires Valid()
-    requires 0 <= i < |Contents|
-    ensures t == Contents[i]
-    decreases Repr
-  {
-    if M <= i {
-      t := elements[i - M];
+    if s.M <= i {
+      t := s.elements.o[i - s.M];
     } else {
-      var arr := more.Get(i / 256);
+      var arr := Get(s.more.o, i / 256);
       t := arr[i % 256];
     }
   }
 
-  method Set(i: int, t: T)
-    requires Valid()
-    requires 0 <= i < |Contents|
-    modifies Repr
-    ensures Valid() && fresh(Repr - old(Repr))
-    ensures Contents == old(Contents)[i := t]
-  {
-    if M <= i {
-      elements := elements[i-M := t];
-    } else {
-      var arr := more.Get(i / 256);
-      arr := arr[i % 256 := t];
-    }
-    Contents := Contents[i := t];
+method Set<T>(s: Eseq<T>, i: int, t: T) returns (s': Eseq<T>)
+  requires Valid(s)
+  requires 0 <= i < |s.Contents|
+  ensures s'.Contents == old(s.Contents)[i := t]
+{
+  s' := s; // duplicate s for modification
+  var Eseq(Contents, elements, more, length, M) := s';
+  if M <= i {
+    s' := Eseq(s'.Contents, Some (s'.elements.o[i - M := t]), s'.more, s'.length, s'.M);
+  } else {
+    var arr := Get(more.o, i / 256);
+    arr := arr[i % 256 := t];
   }
-
-// ~ 4s
-  method Append(t: T)
-    requires Valid()
-    modifies Repr
-    ensures Valid() && fresh(Repr - old(Repr))
-    ensures Contents == old(Contents) + [t]
-    decreases |Contents|
-  {
-    if elements == [] {
-      elements := seq(256, (_ => t));
-      // Repr := Repr + {elements};
-    }
-    if length == 0 || length % 256 != 0 {
-      // there is room in "elements"
-      elements := elements[length - M := t];
-    } else {
-      if more == null {
-        more := new ExtensibleArray.Init();
-        Repr := Repr + {more} + more.Repr;
-      }
-      // "elements" is full, so move it into "more" and allocate a new array
-      more.Append(elements);
-      Repr := Repr + more.Repr;
-      M := M + 256;
-      elements := seq(256, (_ => t));
-      // Repr := Repr + {elements};
-      elements:= elements[0 := t];
-    }
-    length := length + 1;
-    Contents := Contents + [t];
-  }
+  s' := Eseq(Contents[i := t], elements, more, length, M);
 }
+
+method Append<T>(s: Eseq<T>, t: T) returns (s': Eseq<T>)
+  requires Valid(s)
+  ensures s'.Contents == s.Contents + [t]
+  // decreases |s.Contents|
+{
+  s' := s;
+  var Eseq(Contents, elements, more, length, M) := s';
+  if s'.elements == None {
+    s' := Eseq(s'.Contents, Some (seq(256, (_ => t))), s'.more, s'.length, s'.M);
+  }
+  if s'.length == 0 || s'.length % 256 != 0 {
+    // there is room in "elements"
+    s' := Eseq(s'.Contents, Some (s'.elements.o[s'.length - M := t]), s'.more, s'.length, s'.M);
+  } else {
+    if s.more == None {
+      s':= Eseq(s'.Contents, s'.elements, Some(Init()), s'.length, s'.M);
+    }
+    // "elements" is full, so move it into "more" and allocate a new array
+    s' := Append(s'.more.o, s'.elements.o);
+    s' := Eseq(s'.Contents, Some (seq(256, (_ => t))), s'.more, s'.length, s'.M + 256);
+    s' := Eseq(s'.Contents, Some (s'.elements.o[0 := t]), s'.more, s'.length, s'.M);
+  }
+  s' := Eseq(s'.Contents+ [t], s'.elements, s'.more, s'.length+1, s'.M);
+}
+
+// class ExtensibleArray<T> {
+//   ghost var Contents: seq<T>
+//   ghost var Repr: set<object?>
+//   var elements: seq<T>
+//   var more: ExtensibleArray?<seq<T>>
+//   var length: int
+//   var M: int  // shorthand for:  if more == null then 0 else 256 * |more.Contents|
+
+//   predicate Valid()
+//     reads this, Repr
+//   {
+//     // shape of data structure
+//     this in Repr && null !in Repr &&
+//     ((elements == [] && more == null && Contents == []) ||
+//      (elements != [] && |elements| == 256 /*&& elements in Repr*/)) &&
+//     (more != null ==>
+//         more in Repr && more.Repr <= Repr && this !in more.Repr && /*elements !in more.Repr && */
+//         more.Valid() &&
+//         |more.Contents| != 0 &&
+//         forall j :: 0 <= j < |more.Contents| ==>
+//             more.Contents[j] != [] && |more.Contents[j]| == 256 &&
+//             /* more.Contents[j] in Repr && more.Contents[j] !in more.Repr && */
+//             more.Contents[j] != elements &&
+//             forall k :: 0 <= k < |more.Contents| && k != j ==> more.Contents[j] != more.Contents[k]) &&
+
+//     // length
+//     M == (if more == null then 0 else 256 * |more.Contents|) &&
+//     0 <= length <= M + 256 &&
+//     (more != null ==> M < length) &&
+
+//     // Contents
+//     length == |Contents| &&
+//     (forall i :: 0 <= i < M ==> Contents[i] == more.Contents[i / 256][i % 256]) &&
+//     (forall i :: M <= i < length ==> Contents[i] == elements[i - M])
+//   }
+
+//   constructor Init()
+//     ensures Valid() && fresh(Repr - {this})
+//     ensures Contents == []
+//   {
+//     elements := [];
+//     more := null;
+//     length := 0;
+//     M := 0;
+
+//     Contents := [];
+//     Repr := {this};
+//   }
+
+//   method Get(i: int) returns (t: T)
+//     requires Valid()
+//     requires 0 <= i < |Contents|
+//     ensures t == Contents[i]
+//     decreases Repr
+//   {
+//     if M <= i {
+//       t := elements[i - M];
+//     } else {
+//       var arr := more.Get(i / 256);
+//       t := arr[i % 256];
+//     }
+//   }
+
+//   method Set(i: int, t: T)
+//     requires Valid()
+//     requires 0 <= i < |Contents|
+//     modifies Repr
+//     ensures Valid() && fresh(Repr - old(Repr))
+//     ensures Contents == old(Contents)[i := t]
+//   {
+//     if M <= i {
+//       elements := elements[i-M := t];
+//     } else {
+//       var arr := more.Get(i / 256);
+//       arr := arr[i % 256 := t];
+//     }
+//     Contents := Contents[i := t];
+//   }
+
+// // ~ 4s
+//   method Append(t: T)
+//     requires Valid()
+//     modifies Repr
+//     ensures Valid() && fresh(Repr - old(Repr))
+//     ensures Contents == old(Contents) + [t]
+//     decreases |Contents|
+//   {
+//     if elements == [] {
+//       elements := seq(256, (_ => t));
+//       // Repr := Repr + {elements};
+//     }
+//     if length == 0 || length % 256 != 0 {
+//       // there is room in "elements"
+//       elements := elements[length - M := t];
+//     } else {
+//       if more == null {
+//         more := new ExtensibleArray.Init();
+//         Repr := Repr + {more} + more.Repr;
+//       }
+//       // "elements" is full, so move it into "more" and allocate a new array
+//       more.Append(elements);
+//       Repr := Repr + more.Repr;
+//       M := M + 256;
+//       elements := seq(256, (_ => t));
+//       // Repr := Repr + {elements};
+//       elements:= elements[0 := t];
+//     }
+//     length := length + 1;
+//     Contents := Contents + [t];
+//   }
+// }
 
 // method Main() {
 //   var a := new ExtensibleArray.Init();
