SlowTest/NoLongerNeedTest/Lucas-up-trg2.dfy
@@ -147,19 +147,24 @@
 //     }
 //   }
 // }
-function T<A> (x:A) : bool {true}
+// predicate T<A> (x:A) {true} // This one failed
+predicate T (x:nat) {true}
 // z3 with trace=true & proof=true
 lemma INDUCTION_EVEN_ODD(P: (nat, nat) -> bool, a: nat, b: nat)
   requires P(0, 0)
   requires forall a: nat, b: nat :: P(a, b) ==> P(2*a, 2*b)
   requires forall a: nat, b: nat :: P(a, b) ==> P(2*a, 2*b + 1)
   requires forall a: nat, b: nat :: P(a, b) ==> P(2*a + 1, 2*b)
-  requires forall a: nat, b: nat {:trigger T(a), T(b)} :: (T(a) && T(b)) ==> (P(a, b) ==> P(2*a + 1, 2*b + 1))
+  requires forall a: nat, b: nat {:trigger T(a), T(b)} :: T(a) && T(b) && P(a, b) ==> P(2*a + 1, 2*b + 1)
   ensures P(a, b)
 {
   if a == 0 && b == 0 {
   } else {
     INDUCTION_EVEN_ODD(P, a / 2, b / 2);
+    assert a - 1 <= 2 * (a / 2) <= a;
+    assert b - 1 <= 2 * (b / 2) <= b;
+    assert T(a / 2);
+    assert T(b / 2);
   }
 }
 
