SlowTest/SmallestMissingNumber-functional.dfy
@@ -155,6 +155,7 @@ lemma SetEquality(A: set, B: set)
 
 // proof of lemmas supporting proof of main theorem
 
+// element, len, index -> abstract type
 lemma SMN_Correct(xs: List<nat>, n: nat, len: nat)
   requires NoDuplicates(xs)
   requires forall x :: x in Elements(xs) ==> n <= x
